SATsolver/Data/Clause.lean
@@ -1,13 +1,22 @@
 import Std.Data.HashSet
 import SATsolver.Data.Literal
 /-
-  A clause is stored as an array of Literals.
+  A clause is stored as a list of Literals.
   It's logical representation is a disjunction of the
   store literals
 -/
-abbrev Clause : Type := List Lit
+
+def Clause.invariant (c : List Lit) : Prop :=
+  match c with
+  | [] => true
+  | x::xs => x ∉ xs ∧ x.getName ∉ xs.map (fun lit => lit.getName) ∧ invariant xs
+
+structure Clause where
+  lits : List Lit
+  inv : Clause.invariant lits
 
 namespace Clause
+
 
 def toStringHelper (str : String): List Lit → String
   | [] => str
@@ -15,31 +24,29 @@ def toStringHelper (str : String): List Lit → String
   | l :: cs => toStringHelper (str ++ s!"{l} ∨ ") cs
 
 def toString (c : Clause) : String :=
-  toStringHelper "" c
+  toStringHelper "" c.lits
 
 instance : ToString Clause where
   toString x := Clause.toString x
 
-instance : Coe (List Lit) Clause where
-  coe x := (x : Clause)
-
 def subclause (as : Clause)(bs : Clause) : Prop :=
-  ∀ a ∈ as, a ∈ bs
+  ∀ a ∈ as.lits, a ∈ bs.lits
 
 def entails (as : Clause)(bs : Clause) : Bool :=
-  as.all (fun a => bs.contains a)
+  as.lits.all (fun a => bs.lits.contains a)
 
 theorem entails_eq_sub (as : Clause)(bs : Clause) : as.entails bs = true ↔ as.subclause bs := by
   simp [entails, subclause]
 
 def beq (as : Clause)(bs : Clause) : Bool :=
   match as with
-  | [] => match bs with
-    | [] => true
-    | _ :: _ => false
-  | a :: as' => match bs with
-    | [] => false
-    | b :: bs' => a == b ∧ Clause.beq as' bs'
+  | ⟨ [], _ ⟩ => match bs with
+    | ⟨ [], _ ⟩ => true
+    | ⟨ _ :: _, _ ⟩  => false
+  | ⟨ a :: as', inv_a ⟩ => match bs with
+    | ⟨ [], _ ⟩ => false
+    | ⟨ b :: bs', inv_b ⟩ => a == b ∧ Clause.beq ⟨ as', inv_a.right.right ⟩ ⟨ bs', inv_b.right.right⟩
+
 
 @[simp] instance : BEq Clause where
   beq as bs := beq as bs
@@ -47,22 +54,33 @@ def beq (as : Clause)(bs : Clause) : Bool :=
 @[simp] instance : LawfulBEq Clause where
   rfl := by
     intro as
+    rcases as with ⟨ as, inv ⟩
     induction as with
     | nil => simp[beq]
     | cons a as' ih =>
       simp[beq]
       simp at ih
-      exact ih
+      exact ih inv.2.2
   eq_of_beq := by
     intro as bs
+    rcases as with ⟨ as, inv_a ⟩
     induction as generalizing bs with
     | nil =>
-      cases bs <;> simp[beq]
+      rcases bs with ⟨ bs, inv_b ⟩
+      cases bs
+      all_goals simp[beq]
     | cons a as' ih =>
-      cases bs <;> simp[beq]
-      case cons.cons b bs' =>
-        intro lit_h list_h
-        have tail_eq : as' = bs' := ih list_h
-        exact And.intro lit_h tail_eq
+      intro h
+      simp at h
+      rcases bs with ⟨ bs, inv_b ⟩
+      cases bs
+      simp[beq] at h
+      case cons b bs =>
+        simp[beq] at h ⊢
+        constructor
+        exact h.left
+        have := ih inv_a.right.right h.right
+        simp at this
+        exact this
 
 end Clause
