SATsolver/Data/Formula.lean
@@ -1,7 +1,7 @@
 import SATsolver.Data.Clause
 
 
-abbrev Formula : Type := Array Clause
+abbrev Formula : Type := List Clause
 
 namespace Formula
 
@@ -11,11 +11,11 @@ def toStringHelper (str : String): List Clause → String
   | c :: cs => toStringHelper (str ++ s!"{c} ⋀ ") cs
 
 def toString (formula : Formula) : String :=
-  toStringHelper "" formula.toList
+  toStringHelper "" formula
 
 end Formula
 
+def List.toFormula (f : List Clause) : Formula := f
+
 instance : ToString Formula where
   toString x := Formula.toString x
-
-#eval ([(-1 : Int), (2 : Int)] : Clause).contains (Lit.ofInt (-1))
