SATsolver/Data/Trail.lean
@@ -1,114 +1,121 @@
+import Std.Data.HashMap
 import SATsolver.Data.Annotated
-namespace Trail
 
-def uniqueness(stack : List AnnotatedLit) : Prop :=
-  ∀ a ∈ stack, ∀ b ∈ stack, a ≠ b → a.getName ≠ b.getName
+structure Trail.Entry where
+  data : AnnotatedLit
+  prev : Option Nat
 
-def consistency (stack : List AnnotatedLit) (names : Std.HashSet Nat): Prop :=
-  (∀ lit ∈ stack, lit.getName ∈ names) ∧ (∀ name ∈ names, ∃ lit ∈ stack, lit.getName = name)
+instance : Coe Trail.Entry AnnotatedLit where
+  coe a := a.data
+
+@[simp] def Trail.invariant ( entries : Std.HashMap Nat Trail.Entry )(prev : Option Nat) : Prop :=
+  ((exi : prev.isSome) → (prev.get exi) ∈ entries) ∧
+  ∀ n : Nat, (h : n ∈ entries) → ∃ e : Entry, e.data.getName = n ∧ entries[n]'h = e
 
 structure Trail where
-  stack : List AnnotatedLit
-  names : Std.HashSet Nat
-  wf : uniqueness stack ∧ consistency stack names
+  entries : Std.HashMap Nat Trail.Entry
+  prev : Option Nat
+  inv : Trail.invariant entries prev
 
-theorem nin_names_nin_stack (lit : AnnotatedLit)(trail : Trail) :
-  lit.getName ∉ trail.names → lit ∉ trail.stack := by
-    intro h contra
-    apply h
-    cases trail
-    case mk stack names wf =>
-      simp at *
-      have con := wf.right
-      simp[consistency] at con
-      have conL := con.left
-      exact conL lit contra
+namespace Trail
+
+def mem (n : Nat)(as : Trail): Prop :=
+  n ∈ as.entries
+
+instance : Membership Nat Trail where
+  mem as a := Trail.mem a as
 
 def empty : Trail :=
-  have wf : uniqueness [] ∧ consistency [] ∅  := by
-    simp[uniqueness, consistency]
-  {stack := [], names := ∅, wf := wf}
+  ⟨ {}, none, by simp ⟩
 
-def add (as : Trail)(a : AnnotatedLit)(new : a.getName ∉ as.names): Trail :=
-  let stack' := a :: as.stack
-  let names' := as.names.insert a.getName
-  /-Proving invariant-/
-  have wf' : uniqueness stack' ∧ consistency stack' names' := by
-    have new2 := nin_names_nin_stack a as new
+theorem mem_empty (n : Nat) : n ∉ Trail.empty := by
+  simp[empty, Membership.mem]
+  intro contra
+  simp[mem] at contra
+
+def emptyWithCapacity (capacity : Nat) : Trail :=
+  ⟨ Std.HashMap.emptyWithCapacity capacity, none, by simp ⟩
+
+def push (trail : Trail)(lit : AnnotatedLit)(new : lit.getName ∉ trail.entries): Trail :=
+  let entry: Entry := ⟨ lit, trail.prev ⟩
+  let name : Nat := lit.getName
+  let entries' := trail.entries.insert name entry
+  let inv' : invariant entries' (some name) := by
+    simp
+    constructor
+    case left => simp[entries']
+    case right =>
+    intro n nh
+    cases trail
+    case mk entries prev inv =>
+      simp[entries'] at nh
+      cases nh
+      case inl leftH => simp[←leftH, entries', entry, name]
+      case inr rightH =>
+        simp at inv
+        have := inv.right n rightH
+        simp[entries', Std.HashMap.getElem_insert]
+        by_cases name = n
+        case pos posH => simp[posH, entry, name]
+        case neg negH => simp[negH, this]
+  ⟨ entries', some name, inv' ⟩
+
+theorem mem_push (a : AnnotatedLit)(as : Trail)(new : a.getName ∉ as.entries) :
+  a.getName ∈ as.push a new := by
+    simp[push, Membership.mem]
     cases as
-    case mk stack names wf =>
-      simp at *
-      let ⟨ unique, conL, conR ⟩ := wf
-      simp[uniqueness, consistency] at *
-      constructor
-      case left =>
-        intro b bin c cin bnc contra
-        rw[List.mem_cons] at bin cin
-        cases bin
-        case inl bh =>
-          cases cin
-          case inl ch =>
-            apply bnc
-            rw[bh, ch]
-          case inr ch =>
-            apply new
-            simp at ch
-            have cName := conL c ch
-            rw[←bh, contra]
-            exact cName
-        case inr bh =>
-          cases cin
-          case inl ch =>
-            apply new
-            simp at bh
-            have bName := conL b bh
-            rw[←ch, ←contra]
-            exact bName
-          case inr ch =>
-            simp at *
-            apply unique b bh c ch
-            exact bnc
-            exact contra
-      case right =>
-        constructor
-        case left =>
-          intro b bin
-          rw[List.mem_cons] at bin
-          cases bin
-          case inl h =>
-            rw[Std.HashSet.mem_insert, h]
-            left
-            simp
-          case inr h =>
-            simp at h
-            have bn := conL b h
-            rw[Std.HashSet.mem_insert]
-            right
-            exact bn
-        case right =>
-          intro N Nin
-          simp[names'] at Nin
-          cases Nin
-          case inl hl =>
-            exists a
-            constructor
-            rw[List.mem_cons]
-            left
-            rfl
-            exact hl
-          case inr hr =>
-            have h := conR N hr
-            cases h
-            case intro b bh =>
-              exists b
-              constructor
-              case left =>
-                rw[List.mem_cons]
-                right
-                exact bh.left
-              case right =>
-                rw[bh.right]
-  ⟨ stack', names', wf' ⟩
+    case mk as prev inv =>
+      simp[mem]
 
+theorem entry_unique (t : Trail)
+  (n₁ n₂ : Nat)
+  (h₁ : n₁ ∈ t.entries) (h₂ : n₂ ∈ t.entries)
+  (eq_name : (t.entries[n₁]'h₁).data.getName = (t.entries[n₂]'h₂).data.getName) :
+  t.entries[n₁]'h₁ = t.entries[n₂]'h₂ := by
+  -- get witnesses from the invariant
+  have ⟨e₁, he₁_name, he₁_eq⟩ := t.inv.2 n₁ h₁
+  have ⟨e₂, he₂_name, he₂_eq⟩ := t.inv.2 n₂ h₂
+  -- rewrite entries using these witnesses
+  rw [he₁_eq, he₂_eq] at eq_name ⊢
+  -- names correspond to keys
+  rw [he₁_name, he₂_name] at eq_name
+  -- conclude the keys are equal
+  subst eq_name
+  -- now same key: both sides are entries[n₁]
+  simp[←he₁_eq, ←he₂_eq]
+
+
+def satisfies (trail : Trail) (l : Lit) : Prop :=
+  ∃ ann ∈ trail.entries.values, ann.data = l
+
+def falsifies (trail : Trail) (l : Lit) : Prop :=
+  ∃ ann ∈ trail.entries.values, ann.data = -l
+
+def unassigned (trail : Trail) (l : Lit) : Prop :=
+  l.getName ∉ trail.entries
+
+def satisfiesB (trail : Trail) (l : Lit) : Bool :=
+  match trail.entries[l.getName]? with
+  | some ann => ann.data == l
+  | none => false
+
+def falsifiesB (trail : Trail) (l : Lit) : Bool :=
+  match trail.entries[l.getName]? with
+  | some ann => ann.data == -l
+  | none => false
+
+def unassignedB (trail : Trail) (l : Lit) : Bool :=
+  (trail.entries[l.getName]?).isNone
+
+@[simp]
+theorem satisfies_iff_satisfiesB (trail : Trail) (l : Lit) : trail.satisfies l ↔ trail.satisfiesB l := by
+  sorry
+@[simp]
+theorem falsifies_iff_falsifiesB (trail : Trail) (l : Lit) : trail.falsifies l ↔ trail.falsifiesB l := by
+  sorry
+
+@[simp]
+theorem unassigned_iff_unassignedB (trail : Trail) (l : Lit) : trail.unassigned l ↔ trail.unassignedB l := by
+  simp[unassigned, unassignedB]
 
 end Trail
