SATsolver/Assignments.lean
@@ -1,0 +1,484 @@
+import SATsolver.Data.ListTrail
+import SATsolver.Entailment
+
+inductive Status where
+  | sat : Status
+  | fals : Status
+  | undecided : Status
+
+
+
+namespace Trail
+/-
+This file contains interactions between a trail of annotated literals and literals.
+They are used to check whether or not a literal is undecided, satisfied or falsified by a trail.
+-/
+def satisfies (t : Trail)(l : Lit) : Prop :=
+  ∃ a ∈ t.trail, a.getLiteral = l
+
+instance: Entails Trail Lit where
+  entails t l := t.satisfies l
+
+def satisfiesB (t : Trail)(l : Lit) :=
+  match t.get? l with
+  | none => false
+  | some a => a.getLiteral = l
+
+def falsifies (t : Trail)(l : Lit) : Prop :=
+  ∃ a ∈ t.trail, a.getLiteral = -l
+
+def falsifiesB (t : Trail)(l : Lit) :=
+  match t.get? l with
+  | none => false
+  | some a => a.getLiteral = -l
+
+def undecided (t : Trail)(l : Lit) : Prop :=
+  l.getName ∉ t.names
+
+def undecidedB (t : Trail)(l : Lit) :=
+  match t.get? l with
+  | none => true
+  | some _ => false
+
+def decided (t : Trail)(l: Lit) : Prop :=
+  l.getName ∈ t.names
+
+def decidedB (t : Trail)(l : Lit) :=
+  match t.get? l with
+  | none => false
+  | some _ => true
+
+
+@[simp]
+theorem satisfies_iff_satisfiesB (t : Trail)(l : Lit) :
+  t.satisfiesB l = t.satisfies l := by
+  simp[satisfies, satisfiesB]
+  constructor
+  case mp =>
+    intro h; split at h;
+    case h_1 => contradiction
+    case h_2 oe a hget =>
+      simp at h
+      subst h
+      exists a
+      simp
+      exact (get?_eq_some_iff_mem t a).mp hget
+  case mpr =>
+    intro h; cases h;
+    case intro a ah =>
+      have := get?_mems_lit t a ah.left
+      rw[ah.right] at this
+      simp[this, ah.right]
+
+theorem satisfies_not_empty (t : Trail)(l : Lit) :
+  t.satisfies l → t.trail ≠ [] := by
+  simp[satisfies]
+  intro a a_mem h_al
+  exact List.ne_nil_of_mem a_mem
+
+theorem satisfies_subset_satisfies (t : Trail)(l : Lit) :
+  ∀ t', t' ⊆ t → t'.satisfies l → t.satisfies l := by
+  simp[Trail.satisfies]
+  intro t' t'ss a a_mem_t' h_al
+  exists a
+  constructor
+  exact Trail.mem_mem_subset t a t' t'ss a_mem_t'
+  exact h_al
+
+@[simp]
+theorem falsifies_iff_falsifiesB (t : Trail)(l : Lit) :
+  t.falsifiesB l = t.falsifies l := by
+  simp[falsifies, falsifiesB]
+  constructor
+  case mp =>
+    intro h; split at h;
+    case h_1 => contradiction
+    case h_2 oe a hget =>
+      simp at h
+      rw[←get?_eq_get?_neg, ←h] at hget
+      exists a
+      constructor
+      exact (get?_eq_some_iff_mem t a).mp hget
+      exact h
+  case mpr =>
+    intro h; cases h;
+    case intro a ah =>
+    have := get?_mems_lit t a ah.left
+    simp[ah.right] at this
+    simp[this, ah.right]
+
+theorem falsifies_subset_falsifies {t t' : Trail}{l : Lit} :
+  t' ⊆ t → t'.falsifies l → t.falsifies l := by
+  simp[Trail.falsifies]
+  intro t'ss a a_mem_t' h_al
+  exists a
+  constructor
+  exact Trail.mem_mem_subset t a t' t'ss a_mem_t'
+  exact h_al
+
+theorem satisfies_ne_falsifies {t : Trail}{l : Lit}:
+  t.satisfies l → ¬t.falsifies l := by
+  simp[satisfies, falsifies]
+  intro a a_mem h_al x x_mem h_xl
+  have h_al_name := congrArg Lit.getName h_al
+  have h_xl_name := congrArg Lit.getName h_xl
+  simp [AnnotatedLit.simp_getName, Neg.neg, Lit.name_of_neg] at h_al_name h_xl_name
+  rw[←h_al_name] at h_xl_name
+  have := Trail.mem_same_name t x a x_mem a_mem h_xl_name
+  subst this
+  subst h_al
+  exact Lit.neg_ineq x.getLiteral h_xl
+
+
+@[simp]
+theorem undecided_iff_undecidedB (t : Trail)(l : Lit) :
+  t.undecidedB l = t.undecided l := by
+  simp[undecided, undecidedB]
+  constructor
+  case mp =>
+    intro h; split at h;
+    case h_2 => contradiction
+    case h_1 oe h2 =>
+      simp[←get?_some_iff_mem_names, h2]
+  case mpr =>
+    intro h
+    simp[←get?_some_iff_mem_names] at h
+    rw[h]
+
+@[simp]
+theorem decided_iff_decidedB (t : Trail)(l : Lit) :
+  t.decidedB l = t.decided l := by
+    simp[decided, decidedB]
+    constructor
+    case mp =>
+      intro h; split at h;
+      case h_1 => contradiction
+      case h_2 oe a h2 =>
+        simp[←get?_some_iff_mem_names, congrArg Option.isSome h2]
+    case mpr =>
+      intro h
+      simp[←get?_some_iff_mem_names] at h
+      split
+      case h_1 oe noneH =>
+        -- Creates a contradiction
+        rw[noneH] at h
+        simp at h
+      case h_2 oe someH =>
+        simp
+
+@[simp]
+theorem decided_iff_not_undecided{t : Trail}{l : Lit}:
+  ¬t.undecided l ↔ t.decided l:= by
+  simp[undecided, decided]
+
+@[simp]
+theorem decided_iff_sat_or_falsifed (t : Trail)(l : Lit) :
+  t.satisfies l ∨ t.falsifies l ↔ t.decided l  := by
+  simp[decided, satisfies, falsifies]
+  constructor
+  case mp =>
+    intro h
+    cases h
+    case inl satH =>
+      rcases satH with ⟨ a, ⟨ a_mem, a_lit_eq ⟩ ⟩
+      have := t.mem_mem_names a a_mem
+      rw[←a.simp_getName, a_lit_eq] at this
+      exact this
+    case inr falsiH =>
+      rcases falsiH with ⟨ a, ⟨ a_mem, a_lit_neq ⟩ ⟩
+      have := t.mem_mem_names a a_mem
+      rw[←a.simp_getName, a_lit_neq] at this
+      simp[Neg.neg, l.name_of_neg] at this
+      exact this
+  case mpr =>
+    intro h
+    obtain ⟨ a, ⟨ a_mem, aName_eq ⟩ ⟩ := t.names_exi_mem l.getName h
+    rw[←AnnotatedLit.simp_getName] at aName_eq
+    have a_lit := Lit.same_name a.getLiteral l aName_eq
+    cases a_lit
+    case inl aLit_eq => left; exists a;
+    case inr aLit_neq => right; exists a;
+
+theorem sat_iff_not_false_or_u (t : Trail)(l : Lit) :
+  t.satisfies l ↔ ¬t.falsifies l ∧ ¬ t.undecided l := by
+  constructor
+  case mp =>
+    simp[satisfies, falsifies, undecided]
+    cases t
+    case mk t inv =>
+    induction t with
+    | nil => simp
+    | cons x xs ih =>
+      intro a a_mem a_l
+      constructor
+      case left =>
+        intro b b_mem
+        simp at *
+        simp[invariant] at inv
+        cases a_mem; cases b_mem;
+        case inl.inl a_eq b_eq =>
+          rw[b_eq, ←a_eq, a_l]
+          exact Lit.neg_ineq l
+        case inl.inr a_eq b_mem =>
+          rw[←a_eq] at inv
+          have := inv.right.left b b_mem
+          intro contra
+          apply this
+          rw[←a_l] at contra
+          have := congrArg Lit.getName contra
+          simp[Neg.neg] at this
+          exact this
+        cases b_mem;
+        case inr.inl a_mem b_eq =>
+          rw[←b_eq] at inv
+          have := inv.right.left a a_mem
+          intro contra
+          apply this
+          rw[←a_l] at contra
+          have := congrArg Lit.getName contra
+          simp[Neg.neg] at this
+          simp[this]
+        case inr.inr a_mem b_mem =>
+          exact (ih inv.right.right a a_mem a_l).left b b_mem
+      case right =>
+        simp[names] at *
+        rw[←a_l]
+        cases a_mem
+        case inl a_eq => left; simp; exact congrArg AnnotatedLit.getName a_eq
+        case inr a_mem =>
+          right; exists a; constructor
+          exact a_mem
+          simp
+  case mpr =>
+    simp[←decided_iff_sat_or_falsifed]
+    intro not_fals undecided
+    cases undecided
+    case inl sat => exact sat
+    case inr sat => contradiction
+
+theorem false_iff_not_sat_or_u (t : Trail)(l : Lit) :
+  t.falsifies l ↔ ¬t.satisfies l ∧ ¬t.undecided l := by
+  simp[←decided_iff_sat_or_falsifed]
+  constructor
+  case mp =>
+    intro fals
+    constructor
+    case right => right; exact fals
+    case left =>
+       simp[sat_iff_not_false_or_u]
+       intro h
+       contradiction
+  case mpr =>
+    intro ⟨ not_sat, undecided ⟩
+    cases undecided
+    case inl => contradiction
+    case inr fals => exact fals
+
+end Trail
+
+namespace Clause
+
+def satisfiedBy(c :Clause)(t : Trail) :=
+  ∃ l ∈ c.lits, t.satisfies l
+
+def satisfiedByB(c :Clause)(t : Trail) :=
+  c.lits.any (t.satisfiesB .)
+
+@[simp]
+theorem satisfies_iff_satisfiesB (c : Clause)(t : Trail) :
+  c.satisfiedByB t ↔ c.satisfiedBy t := by
+  simp[satisfiedBy, satisfiedByB]
+
+
+def falsifiedBy( c :Clause)(t : Trail) :=
+  ∀ l ∈ c.lits, t.falsifies l
+
+def falsifiedByB( c :Clause)(t : Trail) :=
+  c.lits.all (t.falsifiesB .)
+
+@[simp]
+theorem falsifies_iff_falsifiesB (c : Clause)(t : Trail):
+  c.falsifiedByB t ↔ c.falsifiedBy t := by
+  simp[falsifiedBy, falsifiedByB]
+
+theorem sat_neq_fals {c : Clause}{t : Trail}:
+  c.satisfiedBy t → ¬ c.falsifiedBy t := by
+  simp[satisfiedBy, falsifiedBy]
+  intro l l_mem l_sat
+  exists l
+  constructor
+  exact l_mem
+  exact Trail.satisfies_ne_falsifies l_sat
+
+def undecidedBy (c : Clause)(t : Trail) :=
+  (∃ l ∈ c.lits, t.undecided l) ∧ (∀ l ∈ c.lits, t.undecided l ∨ t.falsifies l)
+
+def undecidedByB (c : Clause)(t : Trail): Bool :=
+  c.lits.any (t.undecidedB .) ∧ c.lits.all (fun l => t.undecidedB l ∨ t.falsifiesB l)
+
+def status (c : Clause)(t : Trail) : Status :=
+  if c.satisfiedByB t then Status.sat
+  else if c.falsifiedByB t then Status.fals
+  else Status.undecided
+
+@[simp]
+theorem undecided_iff_undecidedB(c : Clause)(t : Trail):
+  c.undecidedByB t ↔ c.undecidedBy t := by
+  simp[undecidedBy, undecidedByB]
+
+def unitBy (c : Clause)(t : Trail) :=
+  ∃ l ∈ c.lits, t.undecided l ∧ ∀ k ∈ c.lits, k ≠ l → t.falsifies k
+
+
+def unitByB (c : Clause)(t : Trail) :=
+  let l := c.lits.find? (t.undecidedB .)
+  match l with
+  | none => false
+  | some l => c.lits.all (fun k => k == l ∨ t.falsifiesB k)
+
+@[simp]
+theorem unit_iff_unitBy {c : Clause}{t : Trail}:
+  c.unitByB t ↔ c.unitBy t := by
+  simp[unitBy, unitByB]
+  constructor
+  case mp =>
+    intro h
+    split at h
+    contradiction
+    case h_2 oe l l_find =>
+      simp[List.find?_eq_some_iff_getElem] at *
+      exists l
+      obtain ⟨i, i_wf, l_ind, pre_decided⟩ := l_find.2
+      constructor
+      exact List.mem_of_getElem l_ind
+      constructor
+      exact l_find.1
+      intro k k_mem k_neq
+      exact Or.resolve_left (h k k_mem) k_neq
+  case mpr =>
+    intro h
+    rcases h with ⟨ l, l_mem, l_undecided, mem_h ⟩
+    split
+    case h_1 oe case_h =>
+      simp[Trail.undecided] at case_h l_undecided
+      have := case_h l l_mem
+      contradiction
+    case h_2 oe k k_h =>
+      simp[List.find?_eq_some_iff_getElem] at *
+      obtain ⟨i, i_wf, k_ind, pre_decided⟩ := k_h.2
+      by_cases k_eq : k = l
+      case pos =>
+        subst k_eq
+        intro x x_mem
+        have := mem_h x x_mem
+        by_cases x_eq :x=k
+        left; exact x_eq
+        right; exact this x_eq
+      case neg =>
+        have k_mem := List.mem_of_getElem k_ind
+        have := mem_h k k_mem k_eq
+        simp[t.false_iff_not_sat_or_u] at this
+        have k_decided := this.2
+        have k_undecided := k_h.1
+        contradiction
+
+theorem undecided_if_unit (c : Clause)(t : Trail):
+  c.unitBy t → c.undecidedBy t := by
+  simp[unitBy, undecidedBy]
+  intro l l_mem l_undecided mems_decided
+  constructor
+  exists l
+  intro k k_mem
+  have k_fals := mems_decided k k_mem
+  by_cases k_eq : k = l
+  case pos =>
+    subst k_eq
+    left; exact l_undecided
+  case neg =>
+    right; exact k_fals k_eq
+
+theorem fals_subset_fals {c : Clause}{t t' : Trail}:
+  t ⊆ t' → c.falsifiedBy t → c.falsifiedBy t' := by
+  simp[falsifiedBy]
+  intro ss h l l_mem
+  have : t.falsifies l := h l l_mem
+  exact Trail.falsifies_subset_falsifies ss this
+
+end Clause
+
+namespace Formula
+def satisfiedBy (f : Formula)(t : Trail) : Prop :=
+  (∀ c ∈ f, c.satisfiedBy t)
+
+def is_satisfiedBy (f : Formula)(t : Trail) : Bool :=
+  f.all (fun c => c.satisfiedByB t)
+
+@[simp]
+theorem satisfiedBy_iff_is_satisfiedBy (f : Formula)(t : Trail) :
+  f.is_satisfiedBy t ↔ f.satisfiedBy t := by
+  simp[satisfiedBy, is_satisfiedBy]
+
+def falsifiedBy (f : Formula)(t : Trail) : Prop :=
+  (∃ c ∈ f, c.falsifiedBy t)
+
+def is_falsifiedBy (f : Formula)(t : Trail) : Bool :=
+  f.any (Clause.falsifiedByB . t)
+
+@[simp]
+theorem falsifiedBy_iff_is_falsifiedBy (f : Formula)(t : Trail) :
+  f.is_falsifiedBy t ↔ f.falsifiedBy t := by
+  simp[falsifiedBy, is_falsifiedBy]
+
+def decidedBy (f : Formula)(t : Trail) : Prop :=
+  f.falsifiedBy t ∨ f.satisfiedBy t
+
+theorem decided_head_sat (c : Clause)(cs : Formula)(t : Trail) :
+  c.satisfiedBy t → (c::cs).toFormula.decidedBy t → cs.decidedBy t := by
+  simp[List.toFormula, decidedBy, falsifiedBy, satisfiedBy]
+  intro c_sat h_dec
+  cases h_dec
+  case inl h_fals =>
+    left
+    exact Or.resolve_left h_fals (Clause.sat_neq_fals c_sat)
+  case inr h_sat =>
+    right
+    exact h_sat.right
+
+theorem decided_parts {c : Clause}{cs : Formula}{t : Trail} :
+  c.satisfiedBy t → cs.decidedBy t → (c::cs).toFormula.decidedBy t  := by
+  simp[List.toFormula, decidedBy, falsifiedBy, satisfiedBy]
+  intro c_sat cs_dec
+  cases cs_dec
+  case inl h_fals =>
+    left
+    right
+    exact h_fals
+  case inr h_sat =>
+    right
+    constructor
+    exact c_sat
+    exact h_sat
+
+
+def is_decidedBy (f : Formula)(t : Trail) : Bool :=
+   f.is_falsifiedBy t ∨ f.is_satisfiedBy t
+
+@[simp]
+theorem decidedBy_iff_is_decidedBy (f : Formula)(t : Trail) :
+  f.is_decidedBy t ↔ f.decidedBy t := by
+  simp[is_decidedBy, decidedBy]
+
+def undecidedBy (f : Formula)(t : Trail) : Prop :=
+  ¬ f.decidedBy t
+
+def is_undecidedBy (f : Formula)(t : Trail) : Bool :=
+   ¬ (f.is_falsifiedBy t ∧ f.is_satisfiedBy t)
+
+theorem fals_subset_fals {f : Formula}{t : Trail}{t' : Trail} :
+  t ⊆ t' → f.falsifiedBy t → f.falsifiedBy t' := by
+  simp[falsifiedBy]
+  intro ss c c_mem c_fals
+  exists c
+  constructor
+  exact c_mem
+  exact Clause.fals_subset_fals ss c_fals
