SATsolver/DPLL.lean
@@ -1,0 +1,358 @@
+import SATsolver.Propogation
+
+inductive Clause.state where
+  | fals : state
+  | sat : state
+  | unit :  (c : Clause) → (t : Trail) → c.unitByB t → state
+  | undecided : state
+
+def Clause.getState (c : Clause)(t : Trail) : Clause.state :=
+  if c.falsifiedByB t then Clause.state.fals
+  else if c.satisfiedByB t then Clause.state.sat
+  else if unit : c.unitByB t then Clause.state.unit c t unit
+  else Clause.state.undecided
+
+inductive Formula.state where
+  | conflict : state
+  | sat : state
+  | undecided : List Clause → state
+
+def Formula.getState (f : Formula)(t : Trail) : Formula.state :=
+  let cs : List Clause.state := f.map (fun c => c.getState t)
+  if cs.any (fun s => match s with
+                      | .fals => true
+                      | _  => false ) then Formula.state.conflict
+  else if cs.all (fun s => match s with
+                      | .sat => true
+                      | _  => false ) then Formula.state.sat
+  else
+    let units : List Clause := cs.filterMap (fun s => match s with
+                                                | .unit c  _ _ => some c
+                                                | _ => none )
+    Formula.state.undecided units
+
+def Formula.state.isUndecided (fs : Formula.state) : Prop :=
+  match fs with
+  | undecided _ => True
+  | _ => False
+
+def Formula.state.units (fs : Formula.state)(wf : fs.isUndecided) : List Clause :=
+  match fs with
+  | undecided cs => cs
+
+
+theorem Formula.getState.units_is_units {f: Formula}{t : Trail} :
+    (h : (f.getState t).isUndecided) → ∀ c ∈ (f.getState t).units h, c.unitBy t := by
+    simp[state.isUndecided]
+    intro h c hmem
+    split at h
+    case h_2 => contradiction
+    case h_1 h' fs lc heq =>
+      simp [heq] at hmem
+      simp [state.units] at hmem
+      simp[getState] at heq
+      split at heq
+      case isTrue =>
+        simp at heq -- Sate is conflict -> Contradiction
+      case isFalse =>
+        split at heq
+        case isTrue =>
+          simp at heq -- Sate is sat -> Contradiction
+        case isFalse =>
+          simp at heq
+          rw[←heq] at hmem
+          simp [List.mem_filterMap] at hmem
+          rcases hmem with ⟨ x, ⟨ xmem, h ⟩ ⟩
+          split at h
+          case h_2 => contradiction
+          case h_1 s y t' hunit heq =>
+            simp at h
+            rw[h] at hunit
+            simp[Clause.getState] at heq
+            split at heq
+            contradiction
+            split at heq
+            contradiction
+            split at heq
+            simp at heq
+            simp[←Clause.unit_iff_unitBy, heq, hunit]
+            contradiction
+
+
+
+def SolverState.invariant (ns : List Nat)(t : Trail)(N : Nat) : Prop :=
+  ns.Nodup ∧ (∀ n ∈ ns, n ∉ t.names) ∧ (∀ n ∈ List.range N, n ∈ t.names ∨ n ∈ ns)
+
+structure SolverState where
+  ns : List Nat
+  t : Trail
+  N : Nat
+  inv : SolverState.invariant ns t N
+
+
+theorem SolverState.learn_lit {s : SolverState}{a : AnnotatedLit}{wf : s.ns ≠ []} :
+  a.getName = s.ns.head wf → (unseen : a.getName ∉ s.t.names) → SolverState.invariant s.ns.tail (s.t.push a unseen) s.N := by
+  intro head unseen
+  simp[SolverState.invariant]
+  rcases s with ⟨ ns , t , N, inv ⟩
+  constructor
+  case left =>
+    cases ns
+    case nil => simp
+    case cons x xs => simp [List.nodup_cons.mp inv.1]
+  case right =>
+    constructor
+    case left =>
+      intro m hmem
+      simp[Trail.mem_names_push] at hmem ⊢
+      constructor
+      case left =>
+        cases ns
+        case nil => simp at hmem
+        case cons x xs =>
+          simp at head hmem
+          rw[head]
+          intro contra
+          apply (List.nodup_cons.mp inv.1).left
+          simp[←contra, hmem]
+      case right =>
+        have hmem := List.mem_of_mem_tail hmem
+        exact inv.right.left m hmem
+    case right =>
+      intro m hless
+      have := inv.2.2
+      simp at *
+      have := this m hless
+      cases this
+      simp[Trail.mem_names_push]
+      case inl h =>
+        simp h
+      case inr h =>
+
+
+
+
+namespace DPLL
+
+def decide (s : SolverState)(l : Lit)(k : Nat)
+  (wf : s.ns ≠ [])(head : l.getName = s.ns.head wf): SolverState × Nat :=
+  let a := AnnotatedLit.decided l (k + 1)
+  have unseen : a.getName ∉ s.t.names := by
+    have ln_mem : l.getName ∈ s.ns := by simp[head]
+    have unseen : l.getName ∉ s.t.names := s.inv.2 l.getName ln_mem
+    have : a.getName = l.getName := by simp[a, AnnotatedLit.getName]
+    simp[this, unseen]
+  let t' := s.t.push a unseen
+  let ns' := s.ns.tail
+  have inv' : SolverState.invariant ns' t' := by
+    simp[ns', t']
+    have : l.getName = a.getName := by simp[a, AnnotatedLit.getName]
+    rw[this] at head
+    exact SolverState.learn_lit head unseen
+  ( ⟨ ns', t', s.nLits, inv' ⟩, k+1 )
+
+def forget(s : SolverState)(wf : s.t.trail ≠ []): SolverState :=
+  let a := s.t.trail.head wf
+  let n := a.getName
+  let ns' := n :: s.ns
+  let t' := s.t.pop
+  have inv' : SolverState.invariant ns' t' := by
+    simp[SolverState.invariant, ns']
+    constructor
+    constructor
+    case left.left =>
+      have : n ∈ s.t.names := by
+        have mem : a ∈ s.t.trail := by simp[a]
+        have := Trail.mem_mem_names s.t a mem
+        simp[AnnotatedLit.getName, Lit.getName] at this
+        exact this
+      intro contra
+      apply s.inv.2 n contra
+      exact this
+    case left.right =>
+      exact s.inv.1
+    constructor
+    case right.left =>
+      have : a = s.t.trail.head wf := by rfl
+      have : a.getName ∉ t'.names := Trail.pop_remove_head_name this
+      have hname : n = a.getName := by simp[n, AnnotatedLit.getName, Lit.getName]
+      simp[hname, this]
+    case right.right =>
+      intro m hmem contra
+      have hinv : ¬m ∈ s.t.names := s.inv.2 m hmem
+      have : t' ⊆ s.t := Trail.pop_subset
+      have : m ∈ s.t.names := Trail.names_names_subset this contra
+      contradiction
+  ⟨ ns', t', s.nLits, inv' ⟩
+
+theorem forget_reduces {s : SolverState}{wf : s.t.trail ≠ []} :
+  (forget s wf).t.trail.length < s.t.trail.length := by
+  simp[forget, Trail.pop]
+  have l_neq_zero : s.t.trail.length ≠ 0 := by
+    intro contra
+    rw[List.length_eq_zero_iff] at contra
+    contradiction
+  exact Nat.sub_one_lt l_neq_zero
+
+def backtrack (s : SolverState) (k : Nat) : SolverState × Nat :=
+  if not_nil : ¬s.t.trail.isEmpty then
+    have not_nil : s.t.trail ≠ [] := by
+      simp at not_nil
+      exact not_nil
+    let a := s.t.trail.head not_nil
+    have mem : a ∈ s.t.trail := by simp[a]
+    match hcase : a with
+    | AnnotatedLit.decided (Lit.pos n) m =>
+      let t' := s.t.negate (AnnotatedLit.decided (Lit.pos n) m) mem
+      have inv' : SolverState.invariant s.ns t' := by
+        simp[SolverState.invariant]
+        simp[t', s.inv.1]
+        exact s.inv.2
+      (⟨ s.ns, t', s.nLits, inv' ⟩, m)
+    | AnnotatedLit.decided _ m => backtrack (forget s not_nil) m
+    | _ => backtrack (forget s not_nil) k
+  else ⟨ s, 0 ⟩
+termination_by s.t.trail.length
+  decreasing_by
+  exact forget_reduces
+  exact forget_reduces
+
+theorem List.nodup_erase_nodup {α}[BEq α][LawfulBEq α]{l : List α}{a : α} :
+  l.Nodup → (l.erase a).Nodup := by
+  intro h
+  induction l with
+  | nil => simp
+  | cons x xs ih =>
+    simp[List.erase_cons]
+    split
+    case isTrue =>
+      simp at h
+      exact h.right
+    case isFalse =>
+      simp at *
+      constructor
+      case left hne =>
+        intro contra
+        apply h.left
+        exact (List.mem_erase_of_ne hne).mp contra
+      case right =>
+        exact ih h.right
+
+theorem List.nodup_erase_self_ne_mem {α}[BEq α][LawfulBEq α]{l : List α}(a : α) :
+  l.Nodup → a ∉ (l.erase a) := by
+  intro h
+  induction l with
+  | nil => simp
+  | cons x xs ih =>
+    simp[List.erase_cons]
+    split
+    case isTrue heq =>
+      simp at h heq
+      simp[←heq, h]
+    case isFalse hne =>
+      simp at h hne ⊢
+      constructor
+      case left => intro contra; rw[contra] at hne; contradiction
+      case right => exact ih h.right
+
+
+def propogate (s : SolverState)(c : Clause)(wf : c.unitBy s.t) : SolverState :=
+  let l := c.getUnit s.t wf
+  have undecided : l.getName ∉ s.t.names:= by
+      have : l = c.getUnit s.t wf := by
+          simp[l]
+      exact Clause.getUnit_unseen l wf this
+  let a := AnnotatedLit.propogated l c
+  have unseen : a.getName ∉ s.t.names := by
+      rw[←AnnotatedLit.simp_getName]
+      simp[AnnotatedLit.getLiteral, a]
+      exact undecided
+  let ns' := s.ns.erase l.getName
+  let t' := s.t.push a unseen
+  have inv' : SolverState.invariant ns' t' := by
+    simp[ns', t', SolverState.invariant]
+    rcases s with ⟨ ns, t, _, inv ⟩
+    constructor
+    case left => exact List.nodup_erase_nodup inv.1
+    case right =>
+      simp
+      intro m hmem
+      simp[Trail.mem_names_push] at ⊢
+      constructor
+      case left =>
+        intro contra
+        have hname : l.getName = a.getName := by simp[a, AnnotatedLit.getName]
+        rw[hname, ←contra] at hmem
+        apply List.nodup_erase_self_ne_mem m inv.1
+        exact hmem
+      case right =>
+        have := List.mem_of_mem_erase hmem
+        exact inv.2 m this
+  ⟨ ns', t', s.nLits, inv' ⟩
+
+abbrev Distance : Type := List Nat
+
+def distanceHelper (soFar : Distance) : Nat → List AnnotatedLit → Distance
+  | 0, _  => soFar
+  | n+1, [] => distanceHelper (2::soFar) n []
+  | n+1, a::as => if a.isPos
+                  then distanceHelper (1::soFar) n as
+                  else distanceHelper (0::soFar) n as
+
+def Distance.distance (s : SolverState) : Distance :=
+  (distanceHelper [] s.nLits s.t.trail).reverse
+
+def weightHelper (soFar : Nat) : Distance → Nat
+  | [] => soFar
+  | a :: as => weightHelper (soFar + (a * as.length)) as
+
+def Distance.weight (d : Distance): Nat :=
+  weightHelper 0 d
+
+def Distance.lt : Distance → Distance → Prop
+  | _::_, [] => True
+  | a::as, b::bs => if a < b then True
+                    else if a = b then Distance.lt as bs
+                    else False
+  | [], _ => False
+
+instance : LT Distance where
+  lt as bs := Distance.lt as bs
+
+
+def internal(f : Formula)(s : SolverState)(k : Nat): Formula.state :=
+  let state := f.getState s.t
+  match hs: state with
+  | .conflict =>
+    let ⟨ s', k'⟩ := backtrack s k
+    if k' = 0 then state
+    else internal f s' k'
+  | .sat => state
+  | .undecided unit_cs =>
+    have not_nil : s.ns ≠ [] := by
+      sorry
+    if hempty : unit_cs.isEmpty then internal f (decide s k not_nil) (k+1)
+    else
+      have not_nil : unit_cs ≠ [] := by
+        simp at hempty
+        exact hempty
+      let c := unit_cs.head not_nil
+      have unit_head_unit : c.unitBy s.t := by
+        have state_und : state.isUndecided := by
+          simp[Formula.state.isUndecided, hs]
+        have : (f.getState s.t).units state_und = unit_cs := by
+          simp[Formula.state.units]
+          split
+          case h_1 fs wf cs wf heq₁ heq=>
+            simp [state, heq₁] at hs
+            exact hs
+        have all_units := Formula.getState.units_is_units state_und c
+        have c_mem : c ∈ unit_cs := List.head_mem not_nil
+        simp[this, c_mem] at all_units
+        exact all_units
+      internal f (propogate s c unit_head_unit) k
+termination_by (Distance.distance s).weight
+  decreasing_by
+
+
+def dpll (f : Formula)
