SATsolver/Data.lean
@@ -1,0 +1,5 @@
+/- Import Management file-/
+
+import SATsolver.Data.Clause
+import SATsolver.Data.ListTrail
+import SATsolver.Data.Formula
