SATsolver/Data/ListTrail.lean
@@ -1,0 +1,470 @@
+import SATsolver.data.Annotated
+
+def Trail.invariant (t : List AnnotatedLit): Prop :=
+  match t with
+    | [] => true
+    | x::xs => x ∉ xs ∧ x.getName ∉ xs.map (fun lit => lit.getName) ∧ invariant xs
+
+structure Trail where
+  trail : List AnnotatedLit
+  inv : Trail.invariant trail
+
+namespace Trail
+
+instance : Membership AnnotatedLit Trail where
+  mem t a := a ∈ t.trail
+
+def empty : Trail :=
+  ⟨ [], by simp[invariant] ⟩
+
+def lits (t : Trail) : List Lit :=
+  t.trail.map (fun a => a.getLiteral)
+
+theorem mem_mem_lits (t : Trail)(a : AnnotatedLit):
+  a ∈ t.trail → a.getLiteral ∈ t.lits := by
+  simp[lits]
+  induction t.trail with
+  | nil => simp
+  | cons x xs ih =>
+    simp; intro h; cases h
+    case inl h => left; simp[h]
+    case inr h => right; exact ih h
+
+theorem not_lits_not_mem(t : Trail)(a : AnnotatedLit):
+  a.getLiteral ∉ t.lits → a ∉ t.trail := by
+  simp[lits]
+  induction t.trail with
+  | nil => simp
+  | cons x xs ih =>
+    simp; intro ineq lit_ineq
+    constructor
+    intro contra; apply ineq; simp[contra]
+    exact ih lit_ineq
+
+theorem lits_exi_mem(t : Trail)(l : Lit):
+  l ∈ t.lits → ∃ a ∈ t.trail, a.getLiteral = l := by
+  cases t
+  case mk t inv =>
+    induction t with
+    | nil => simp[lits]
+    | cons x xs ih =>
+      simp[lits]; intro h; cases h
+      case inl leftH => left; simp[leftH]
+      case inr rightH => right; exact rightH
+
+def names (t : Trail) : List Nat :=
+  t.trail.map (fun a => a.getName)
+
+theorem mem_mem_names (t : Trail)(a : AnnotatedLit):
+  a ∈ t.trail → a.getName ∈ t.names := by
+  simp[names]
+  induction t.trail with
+  | nil => simp
+  | cons x xs ih =>
+    simp; intro h; cases h
+    case inl h => left; simp[h]
+    case inr h => right; exact ih h
+
+theorem not_names_not_mem(t : Trail)(a : AnnotatedLit):
+  a.getName ∉ t.names → a ∉ t.trail := by
+  simp[names]
+  induction t.trail with
+  | nil => simp
+  | cons x xs ih =>
+    simp; intro ineq name_ineq
+    constructor
+    intro contra; apply ineq; simp[contra]
+    exact ih name_ineq
+
+theorem names_exi_mem(t : Trail)(n : Nat):
+  n ∈ t.names → ∃ a ∈ t.trail, a.getName = n := by
+  cases t
+  case mk t inv =>
+    induction t with
+    | nil => simp[names]
+    | cons x xs ih =>
+      simp[names]; intro h; cases h
+      case inl leftH => left; simp[leftH]
+      case inr rightH => right; exact rightH
+
+theorem mem_same_name (t : Trail)(a b : AnnotatedLit) :
+  a ∈ t.trail → b ∈ t.trail → a.getName = b.getName → a = b := by
+  intro a_mem b_mem name_eq
+  rcases t with ⟨ trail, inv ⟩
+  induction trail with
+  | nil => simp at *
+  | cons x xs ih =>
+    simp at *
+    cases a_mem; cases b_mem
+    case inl.inl ha hb =>
+      rw[ha, hb]
+    case inl.inr ha hb =>
+      subst ha
+      have := inv.2.1
+      simp at this
+      have := this b hb
+      symm at name_eq
+      contradiction
+    cases b_mem
+    case inr.inl ha hb =>
+      subst hb
+      have := inv.2.1
+      simp at this
+      have := this a ha
+      contradiction
+    case inr.inr ha hb =>
+      exact ih inv.2.2 ha hb
+
+
+def get? (t : Trail)(l : Lit) : Option AnnotatedLit :=
+  t.trail.find? (fun a => a.getName = l.getName)
+
+
+@[simp]
+theorem get?_some_iff_mem_names (t : Trail)(l : Lit) :
+  (t.get? l).isSome = true ↔ l.getName ∈ t.names := by
+  simp[get?]
+  constructor
+  intro h; cases h;
+  case intro a ah =>
+    rw[←ah.right]
+    exact mem_mem_names t a ah.left
+  intro h
+  exact names_exi_mem t l.getName h
+
+theorem get?_mems_lit (t : Trail)(a : AnnotatedLit):
+  a ∈ t.trail → t.get? a.getLiteral = some a := by
+  cases t
+  case mk trail inv =>
+  simp[get?]
+  induction trail with
+  | nil => simp
+  | cons x xs ih =>
+    intro h; simp at h ⊢;
+    have name_inv : ∀ (x_1 : AnnotatedLit), x_1 ∈ xs → ¬x_1.getName = x.getName := by
+      simp[invariant] at inv
+      exact inv.right.left
+    cases h
+    case inl leftH => left; simp[leftH]
+    case inr rightH =>
+      right
+      constructor
+      case left =>
+        have := name_inv a rightH
+        intro contra; apply this; simp[contra]
+      case right =>
+        have := inv.2.2
+        exact ih this rightH
+
+theorem get?_lits_some_val (t : Trail)(l : Lit) :
+  l ∈ t.lits → ∃ a, t.get? l = some a := by
+  intro h
+  obtain ⟨ a, ah ⟩ := lits_exi_mem t l h
+  exists a
+  rw[←ah.right]
+  apply get?_mems_lit
+  exact ah.left
+
+theorem get?_names_some_val (t : Trail)(n : Nat) :
+  n ∈ t.names → ∃ a l, l.getName = n → t.get? l = some a := by
+  intro h
+  obtain ⟨ a, ah ⟩ := t.names_exi_mem n h
+  have := t.mem_mem_lits a ah.left
+  exists a
+  exists a.getLiteral
+  simp[ah.right]
+  exact t.get?_mems_lit a ah.left
+
+
+theorem get?_eq_some_mem {l} (t : Trail)(a : AnnotatedLit):
+  t.get? l = some a → a ∈ t.trail := by
+  cases t
+  case mk trail inv =>
+  simp[get?]
+  induction trail with
+  | nil => simp
+  | cons x xs ih =>
+    intro h
+    simp at h
+    cases h
+    case inl leftH => simp[←leftH.right]
+    case inr rightH => simp[ih inv.right.right rightH.right]
+
+@[simp]
+theorem get?_eq_some_iff_mem (t : Trail)(a : AnnotatedLit):
+  t.get? a.getLiteral = some a ↔ a ∈ t.trail := by
+  constructor
+  exact get?_eq_some_mem t a
+  exact get?_mems_lit t a
+
+@[simp]
+theorem get?_eq_get?_neg (t : Trail)(l : Lit):
+  t.get? (-l) = t.get? l := by
+  simp[get?, Neg.neg]
+
+def push (t : Trail)(a : AnnotatedLit)(wf : a.getName ∉ t.names) : Trail :=
+  let t' := a::t.trail
+  let inv' : invariant t' := by
+    unfold invariant
+    constructor
+    case left => exact not_names_not_mem t a wf
+    constructor
+    case right.left =>
+      simp; intro b b_mem;
+      have b_name_mem := mem_mem_names t b b_mem
+      intro contra
+      rw[contra] at b_name_mem
+      contradiction
+    case right.right => exact t.inv
+  ⟨ t', inv'⟩
+
+theorem mem_push {t : Trail}{a b: AnnotatedLit}{wf : b.getName ∉ t.names} :
+  a ∈ (t.push b wf).trail ↔ a = b ∨ a ∈ t.trail  := by
+  simp[push]
+
+theorem mem_names_push {t : Trail}{a : AnnotatedLit}{n : Nat}{wf : a.getName ∉ t.names} :
+  n ∈ (t.push a wf).names ↔ n = a.getName ∨ n ∈ t.names := by
+  simp[push, names]
+
+
+def pop (t : Trail) : Trail :=
+  have inv : Trail.invariant t.trail.tail := by
+    rcases t with ⟨ trail, inv ⟩
+    simp[List.tail]
+    split
+    case h_1 => simp[invariant]
+    case h_2 _ x xs =>
+      exact inv.2.2
+  ⟨ t.trail.tail, inv ⟩
+
+theorem pop_remove_head {t : Trail}{a : AnnotatedLit}{wf : t.trail ≠ []}:
+  a = t.trail.head wf → a ∉ t.pop := by
+  simp[pop]
+  intro hhead
+  rcases t with ⟨ trail, inv ⟩
+  cases trail
+  case nil => contradiction
+  case cons b bs =>
+    simp at *
+    subst hhead
+    exact inv.1
+
+theorem pop_remove_head_name {t : Trail}{a : AnnotatedLit}{wf : t.trail ≠ []}:
+  a = t.trail.head wf → a.getName ∉ t.pop.names := by
+  simp[pop, names]
+  intro hhead
+  rcases t with ⟨ trail, inv ⟩
+  cases trail
+  case nil => contradiction
+  case cons b bs =>
+    have := inv.2.1
+    simp at *
+    subst hhead
+    exact this
+
+theorem inv_new_head_same_name {a b : AnnotatedLit}{as : List AnnotatedLit} :
+  a.getName = b.getName → invariant (a::as) → invariant (b::as) := by
+    unfold invariant
+    intro hname a_inv
+    have bname : ¬b.getName ∈ List.map (fun lit => lit.getName) as := by
+      rw[hname] at a_inv
+      exact a_inv.2.1
+    constructor
+    case left =>
+      intro contra
+      apply bname
+      exact List.mem_map_of_mem contra
+    case right =>
+      constructor
+      exact bname
+      exact a_inv.2.2
+
+theorem replace_no_dup {α}[BEq α] {a b c: α}{as : List α} :
+  a ∉ as → a ≠ c → a ∉ as.replace b c := by
+  intro hmem heq contra
+  induction as with
+  | nil => simp at contra
+  | cons x xs ih =>
+    simp[List.replace_cons] at contra
+    by_cases hbeq : b==x
+    case pos =>
+      simp[hbeq] at contra hmem
+      have hamem := hmem.right
+      cases contra
+      all_goals contradiction
+    case neg =>
+      simp[hbeq] at contra hmem
+      have ⟨ haeq, hamem ⟩ :=  hmem
+      rcases contra with _ | hmem_replace
+      contradiction
+      exact ih hamem hmem_replace
+
+theorem replace_mem {α}[BEq α]{a b c: α}{as : List α} :
+  a ∈ as.replace b c → a ∈ as ∨ a = c := by
+  intro h
+  induction as with
+  | nil => simp at h
+  | cons x xs ih =>
+    simp[List.replace_cons] at h
+    by_cases heq : b == x
+    case pos =>
+      simp [heq] at h
+      rcases h with heq | hmem
+      case inl => simp[heq]
+      case inr => simp[hmem]
+    case neg =>
+      simp[heq] at h
+      rcases h with heq | hmem
+      case inl => simp[heq]
+      case inr =>
+        simp[hmem] at ih
+        rcases ih with hmem | heq
+        case inl => simp [hmem]
+        case inr => simp[heq]
+
+
+theorem inv_replace {a b : AnnotatedLit}{as : List AnnotatedLit} :
+  invariant as → a.getName = b.getName → invariant (as.replace a b) := by
+  intro inv hname
+  induction as with
+  | nil => simp[inv]
+  | cons x xs ih =>
+    by_cases hmem : a ∈ x::xs
+    case neg =>
+      rw[List.replace_of_not_mem hmem]
+      exact inv
+    case pos =>
+      rw[List.replace_cons]
+      by_cases heq₂ : a == x
+      case pos =>
+        simp at heq₂
+        simp [heq₂]
+        rw[←heq₂] at inv
+        exact inv_new_head_same_name hname inv
+      case neg =>
+        simp[heq₂, inv.2.2] at ⊢ ih
+        simp at heq₂
+        simp[heq₂] at hmem
+        have hname₂ : a.getName ≠ x.getName := by
+          have := inv.2.1
+          simp at this
+          exact this a hmem
+        rw[hname] at hname₂
+        have heq₃ : b ≠ x := AnnotatedLit.name_ineq hname₂
+        symm at heq₃
+        unfold invariant
+        constructor
+        case left =>
+          have := inv.1
+          exact replace_no_dup this heq₃
+        case right =>
+          constructor
+          case left =>
+            simp
+            intro y hmem₂
+            have := replace_mem hmem₂
+            rcases this with hmem₃ | heq₄
+            case inl =>
+              have := inv.2.1
+              simp at this
+              exact this y hmem₃
+            case inr =>
+              subst heq₄
+              exact hname₂
+          case right =>
+            exact ih
+
+def negate (t : Trail)(a : AnnotatedLit)(wf : a ∈ t.trail) : Trail :=
+  let negated := a.negate
+  let trail' := t.trail.replace a negated
+  have inv' : invariant trail' := by
+    have hname : a.getName = a.negate.getName := AnnotatedLit.name_negated
+    rcases t with ⟨ trail, inv ⟩
+    simp[trail']
+    exact inv_replace inv hname
+    ⟨ trail', inv' ⟩
+
+theorem map_replace_eq_self_of_eq{l : List AnnotatedLit}{a b : AnnotatedLit}{f : AnnotatedLit → Nat}:
+  f a = f b → (l.replace a b).map f = l.map f := by
+  intro hfeq
+  induction l with
+  | nil => simp
+  | cons x xs ih =>
+    simp[List.replace_cons]
+    split
+    case h_1 _ heq =>
+      simp at heq
+      simp[List.map]
+      rw[←hfeq, ←heq]
+    case h_2 _ heq =>
+      simp[ih]
+
+
+@[simp]
+theorem names_negate {t : Trail}{a : AnnotatedLit}{mem : a ∈ t.trail} :
+  (t.negate a mem).names = t.names := by
+  simp[negate]
+  have hname : a.getName = a.negate.getName := AnnotatedLit.name_negated
+  rcases t with ⟨ trail, inv ⟩
+  have : (trail.replace a a.negate).map AnnotatedLit.getName = trail.map AnnotatedLit.getName := map_replace_eq_self_of_eq hname
+  simp[names, this]
+
+
+instance : HasSubset Trail where
+  Subset sub super := ∀ x ∈ sub.trail, x ∈ super.trail
+
+theorem subset_empty (t : Trail):
+  t ⊆ empty ↔ t = empty := by
+  simp[HasSubset.Subset, empty]
+  rcases t with ⟨ trail, inv ⟩
+  constructor
+  case mp =>
+    intro h
+    simp[List.eq_nil_iff_forall_not_mem, h]
+  case mpr =>
+    intro h
+    simp at *
+    simp[h]
+
+theorem subset_self (t : Trail):
+  t ⊆ t := by
+  simp[HasSubset.Subset]
+
+theorem subset_push_self(t : Trail):
+  ∀ a (wf : a.getName ∉ t.names), t ⊆ t.push a wf := by
+  simp[push]
+  intro a a_new x x_mem
+  simp[x_mem]
+
+theorem mem_mem_subset(t : Trail)(a : AnnotatedLit):
+  ∀ t', t' ⊆ t → a ∈ t' → a ∈ t := by
+  simp[HasSubset.Subset]
+  intro t' t'ss a_mem_t'
+  exact t'ss a a_mem_t'
+
+theorem lits_lits_subset{t t': Trail}{l : Lit}:
+  t' ⊆ t → l ∈ t'.lits → l ∈ t.lits := by
+  simp[lits]
+  intro t'ss a a_mem_t' h_al
+  exists a
+  constructor
+  exact mem_mem_subset t a t' t'ss a_mem_t'
+  exact h_al
+
+theorem names_names_subset {t t': Trail}{n : Nat}:
+  t' ⊆ t → n ∈ t'.names → n ∈ t.names := by
+  simp[names]
+  intro t'ss a a_mem_t' h_an
+  exists a
+  constructor
+  exact mem_mem_subset t a t' t'ss a_mem_t'
+  exact h_an
+
+theorem pop_subset {t : Trail}:
+  t.pop ⊆ t := by
+  simp[pop, HasSubset.Subset, List.tail]
+  intro x hmem
+  split at hmem
+  case h_1 => contradiction
+  case h_2 _ a as heq =>
+    simp[heq, hmem]
