SATsolver/Entailment.lean
@@ -1,4 +1,4 @@
-import SATsolver.Literal
+import SATsolver.Data
 
 class Entails (α β : Type) where
   entails : α → β → Prop
@@ -7,13 +7,13 @@ infix:50 "⊨" => Entails.entails
 infix:50 "⊭" => ¬Entails.entails
 
 instance : Entails Lit Clause where
-  entails l c := l ∈ c
+  entails l c := l ∈ c.lits
 
 instance : Entails AnnotatedLit Clause where
-  entails al c := al.getLiteral ∈ c
+  entails al c := al.getLiteral ∈ c.lits
 
-instance : Entails Tail Clause where
+instance : Entails Trail Clause where
   entails tl c := ∃ al ∈ tl, al ⊨ c
 
-instance : Entails Tail Formula where
+instance : Entails Trail Formula where
   entails tl f := ∀ c ∈ f, tl ⊨ c
