SATsolver/Propogation.lean
@@ -1,0 +1,58 @@
+import SATsolver.Assignments
+
+theorem Clause.unit_elim (c : Clause)(t : Trail) :
+    ∀ l : Lit, c.unitBy t ∧ t.undecided l ∧ l ∈ c.lits
+    → ∀ t', t ⊆ t' → c.satisfiedBy t' = t'.satisfies l := by
+    intro l lh t' t'SS
+    simp[Clause.unitBy] at lh
+    have ⟨ c_unit_t, l_undecided_t, l_mem_c ⟩ := lh
+    rcases c_unit_t with ⟨ j, j_mem_c, j_undecided_t, non_j_fals ⟩
+    by_cases l_eq_j : l = j
+    case neg =>
+        have := non_j_fals l l_mem_c l_eq_j
+        have t_decided_l : t.decided l := by
+            rw[←Trail.decided_iff_sat_or_falsifed]
+            right; exact this
+        contradiction
+    subst l_eq_j
+    apply iff_iff_eq.mp
+    constructor
+    case pos.mp =>
+        intro c_sat_t'
+        simp[Clause.satisfiedBy] at c_sat_t'
+        rcases c_sat_t' with ⟨ j, ⟨ j_mem, t'sat_j ⟩ ⟩
+        by_cases l_eq_j : j = l
+        case neg =>
+            have := non_j_fals j j_mem l_eq_j
+            have := Trail.falsifies_subset_falsifies t'SS this
+            have := Trail.satisfies_ne_falsifies t'sat_j
+            contradiction
+        subst l_eq_j
+        exact t'sat_j
+    case pos.mpr =>
+        intro t'sat_l
+        simp[satisfiedBy]
+        exists l
+
+def Clause.getUnit (c : Clause)(t : Trail)(wf : c.unitBy t) : Lit :=
+    let l := c.lits.find? (fun l => t.undecidedB l)
+    have is_some : l.isSome := by
+        simp[←Clause.unit_iff_unitBy, Clause.unitByB] at wf
+        split at wf
+        case h_1 => contradiction
+        case h_2 _ _ h => simp[l, h]
+    l.get is_some
+
+theorem Clause.getUnit_unseen {c : Clause}{t : Trail}(l : Lit)
+    (wf : c.unitBy t) :
+    l = c.getUnit t wf → t.undecided l := by
+    intro h
+    simp[←Clause.unit_iff_unitBy, Clause.unitByB, getUnit] at wf h
+    split at wf
+    case h_1 => contradiction
+    case h_2 _ k h_k =>
+        simp[h_k] at h
+        have := List.find?_some h_k
+        simp at this
+        subst h
+        exact this
